src/3d/Translate.fsti
@@ -21,4 +21,4 @@ module B = Binding
 module T = Target
 open FStar.All
 
-val translate_decls (env:B.global_env) (d:list A.decl) : ML (list T.decl)
+val translate_decls (env:B.global_env) (senv:TypeSizes.env_t) (d:list A.decl) : ML (list T.decl)
