src/3d/TypeSizes.fst
@@ -1,0 +1,251 @@
+(*
+   Copyright 2019 Microsoft Research
+
+   Licensed under the Apache License, Version 2.0 (the "License");
+   you may not use this file except in compliance with the License.
+   You may obtain as copy of the License at
+
+       http://www.apache.org/licenses/LICENSE-2.0
+
+   Unless required by applicable law or agreed to in writing, software
+   distributed under the License is distributed on an "AS IS" BASIS,
+   WITHOUT WARRANTIES OR CONDITIONS OF ANY KIND, either express or implied.
+   See the License for the specific language governing permissions and
+   limitations under the License.
+*)
+module TypeSizes
+open FStar.All
+open Ast
+open FStar.Mul
+module H = Hashtable
+module B = Binding
+
+let product_size (base:size) (n:int) =
+  match base with
+  | Variable
+  | WithVariableSuffix _ ->
+    Variable
+  | Fixed k ->
+    Fixed (k * n)
+
+let typename = string
+
+let size_env = H.t typename size
+
+let initial_env (benv:B.global_env) : ML env_t =
+  let i = [
+       ("unit",     Fixed 0);
+       ("Bool",     Fixed 1);
+       ("UINT8",    Fixed 1);
+       ("UINT16",   Fixed 2);
+       ("UINT32",   Fixed 4);
+       ("UINT64",   Fixed 8);
+       ("field_id", Fixed 4);
+       ("PUINT8",   Variable) //size of pointer is platform-dependent
+  ]
+  in
+  let senv = H.create 17 in
+  List.iter (fun (i, k) -> H.insert senv i k) i;
+  B.mk_env benv,
+  senv
+
+let size_of_typename (env:env_t) (i:ident)
+  : ML size
+  = match H.try_find (snd env) i.v with
+    | Some s -> s
+    | None -> failwith (Printf.sprintf "size_of_typename: Identifier %s not found" i.v)
+
+let extend_with_size_of_ident (env:env_t) (i:ident) (n:size)
+  : ML unit
+  = H.insert (snd env) i.v n
+
+let extend_with_size_of_typedef_names (env:env_t) (names:typedef_names) (size:size)
+  : ML unit
+  = extend_with_size_of_ident env names.typedef_name size;
+    extend_with_size_of_ident env names.typedef_abbrev size;
+    extend_with_size_of_ident env names.typedef_ptr_abbrev Variable
+
+let size_of_typ (env:env_t) (t:typ)
+  : ML size
+  = match t.v with
+    | Type_app i _ -> size_of_typename env i
+    | Pointer _ -> Variable
+
+let rec value_of_const_expr (env:env_t) (e:expr)
+  : ML (option (either bool (integer_type & int)))
+  =
+  match e.v with
+  | Constant (Int t n) -> Some (Inr (t, n))
+  | Constant (Bool b) -> Some (Inl b)
+  | App op [e1; e2] ->
+    let v1 = value_of_const_expr env e1 in
+    let v2 = value_of_const_expr env e2 in
+    begin
+    match op, v1, v2 with
+    | Plus _,  Some (Inr (t1, n1)), Some (Inr (t2, n2)) -> Some (Inr (integer_type_lub t1 t2, n1 + n2))
+    | Minus _, Some (Inr (t1, n1)), Some (Inr (t2, n2)) -> Some (Inr (integer_type_lub t1 t2, n1 - n2))
+    | Mul _,   Some (Inr (t1, n1)), Some (Inr (t2, n2)) -> Some (Inr (integer_type_lub t1 t2, n1 * n2))
+    | Division _, Some (Inr (t1, n1)), Some (Inr (t2, n2)) ->
+      if n2 = 0
+      then error ("Division by zero in constant expression") e2.range
+      else Some (Inr (integer_type_lub t1 t2, n1 / n2))
+    | GT _, Some (Inr (_, n1)), Some (Inr (_, n2)) -> Some (Inl (n1 > n2))
+    | LT _, Some (Inr (_, n1)), Some (Inr (_, n2)) -> Some (Inl (n1 < n2))
+    | GE _, Some (Inr (_, n1)), Some (Inr (_, n2)) -> Some (Inl (n1 >= n2))
+    | LE _, Some (Inr (_, n1)), Some (Inr (_, n2)) -> Some (Inl (n1 <= n2))
+    | And, Some (Inl b1), Some (Inl b2) -> Some (Inl (b1 && b2))
+    | Or, Some (Inl b1), Some (Inl b2) -> Some (Inl (b1 || b2))
+    | _ -> None
+    end
+  | App Not [e] ->
+    let v = value_of_const_expr env e in
+    begin
+    match v with
+    | Some (Inl b) -> Some (Inl (not b))
+    | _ -> None
+    end
+  | App SizeOf [{v=Identifier t}] ->
+    begin
+    try
+      match size_of_typ env (with_range (Type_app t []) t.range) with
+      | Fixed n
+      | WithVariableSuffix n -> Some (Inr (UInt32, n))
+      | _ -> None
+    with
+      | _ -> None
+    end
+  | App (Cast _ t) [e] ->
+    let v = value_of_const_expr env e in
+    begin
+    match v with
+    | Some (Inr (_, n)) ->
+      Some (Inr (t, n))
+    | _ -> None
+    end
+  | Identifier i ->
+    begin
+    match B.lookup_macro_definition (fst env) i with
+    | Some e ->
+      value_of_const_expr env e
+    | _ -> None
+    end
+  | _ -> None
+
+let size_of_field (env:env_t) (f:field)
+  : ML size
+  = let base_size = size_of_typ env f.v.field_type in
+    match f.v.field_array_opt with
+    | None ->
+      base_size
+
+    | Some (e, ConstantSize) ->
+      let n = value_of_const_expr env e in
+      begin
+      match n with
+      | Some (Inr (_, k)) ->
+        product_size base_size k
+
+      | _ ->
+        error (Printf.sprintf "Constant sized array expression %s could not be statically evaluated to a constant"
+                                (print_expr e))
+              f.range
+      end
+
+    | Some (n, VariableSizeEq)
+    | Some (n, SingleElementVariableSizeEq) ->
+      let n = value_of_const_expr env n in
+      begin
+      match n with
+      | Some (Inr (_, k)) ->
+        product_size base_size k
+
+      | _ ->
+        Variable
+      end
+
+    | _ -> Variable
+
+let size_of_decl (env:env_t) (d:decl)
+  : ML unit
+  = match d.v with
+    | Define _ _ _ -> ()
+
+    | TypeAbbrev t i
+    | Enum t i _ ->
+      extend_with_size_of_ident env i (size_of_typ env t)
+
+    | Record names params where fields ->
+      let field_sizes = List.map (size_of_field env) fields in
+      let size =
+        List.fold_right
+          (fun f_size accum ->
+            match accum with
+            | None -> //f is the last field
+              begin
+              match f_size with
+              | Fixed _
+              | WithVariableSuffix _ ->
+                Some f_size
+              | Variable ->
+                Some (WithVariableSuffix 0)
+              end
+            | Some s_suffix ->
+              let s =
+                match f_size, s_suffix with
+                | Variable, _
+                | WithVariableSuffix _, _ ->
+                  Variable
+
+                | Fixed n0, Fixed n1 ->
+                  Fixed (n0 + n1)
+
+                | Fixed n0, WithVariableSuffix n ->
+                  WithVariableSuffix (n0 + n)
+
+                | Fixed _, Variable ->
+                  Variable
+              in
+              Some s)
+          field_sizes
+          None
+      in
+      let size =
+        match size with
+        | None -> Fixed 0 //empty record
+        | Some s -> s
+      in
+      extend_with_size_of_typedef_names env names size
+
+    | CaseType names params cases ->
+      let case_sizes =
+        List.map
+          (function
+            | Case _ f
+            | DefaultCase f ->
+              size_of_field env f)
+          (snd cases)
+      in
+      let size =
+        List.fold_right
+          (fun s accum ->
+            match accum with
+            | None -> Some s
+            | Some s' ->
+              if s = s'
+              then Some s
+              else Some Variable)
+          case_sizes
+          None
+      in
+      let size =
+        match size with
+        | None -> Fixed 0
+        | Some s -> s
+      in
+      extend_with_size_of_typedef_names env names size
+
+let size_of_decls (env:B.global_env) (d:list decl)
+  : ML env_t
+  = let env = initial_env env in
+    List.iter (size_of_decl env) d;
+    env
